lean/AbsDen.lean
@@ -5,7 +5,7 @@ import AbsDen.Env
 import AbsDen.Semantics
 import AbsDen.Trace
 import AbsDen.LR
+import AbsDen.AbstractDomain
 import AbsDen.ByName
 import AbsDen.ByNeed
 import AbsDen.NoConsecInvis
-import AbsDen.LRGood
